src/high/dprop.v
@@ -6,28 +6,41 @@ From iris.proofmode Require Import monpred tactics.
 From iris.base_logic.lib Require Import iprop.
 
 From self Require Export view memory.
+From self.high Require Export resources.
+
+Instance subseteq_nvmdeltag : SqSubsetEq nvmDeltaG := λ v w, v = w.
+
+Instance nvmDeltaG_inhabited : Inhabited (nvmDeltaG).
+Proof. repeat split; apply 1%positive. Qed.
+
+(* Our propositions are parameterized by a thread view and a record of ghost names.
+   For now we call this type [index] and use [i] to range over it.
+ *)
+Notation index := (thread_view * nvmDeltaG)%type.
 
 (* We define a canonical [biIndex] structure for [thread_view]. All fields except for
 [bi_index_type] can be infered by Coq. *)
 Canonical Structure thread_view_bi_index : biIndex :=
-  {| bi_index_type := thread_view; |}.
+  {| bi_index_type := index; |}.
 
 (* Uncomment this to see the fields that Coq infer. *)
 (* Print thread_view_bi_index. *)
 
+(*
 Instance view_bi_index_bot (TV : thread_view) : BiIndexBottom (ε : thread_view).
 Proof.
   rewrite /BiIndexBottom. intros [[??] ?]. rewrite !subseteq_prod'.
   rewrite !subseteq_view_incl.
   split; first split; apply: ucmra_unit_least.
 Qed.
+*)
 
 (* Types of view predicates. *)
 Definition dProp Σ := monPred thread_view_bi_index (iPropI Σ).
 Definition dPropO Σ := monPredO thread_view_bi_index (iPropI Σ).
 Definition dPropI Σ := monPredI thread_view_bi_index (iPropI Σ).
 
-Ltac iModel := iStartProof (iProp _); iIntros (TV).
+Ltac iModel := iStartProof (iProp _); iIntros ([TV gnames]).
 
 (* [bi_scope] is the scope associated with the scope key [I] from Iris. We bind
 it to the [dProp] type such that we avoid having to type `%I` to get the right
@@ -37,23 +50,34 @@ Bind Scope bi_scope with dProp.
 Section definitions.
   Context {Σ : gFunctors}.
 
+  Program Definition have_thread_view (TV : thread_view) : dProp Σ:=
+    MonPred (λ i, ⌜ TV ⊑ i.1 ⌝%I) _.
+  Next Obligation. solve_proper. Qed.
+
+  Global Instance have_thread_view_persistent TV1 :
+    Persistent (have_thread_view TV1).
+  Proof. rewrite /Persistent. iModel. auto. Qed.
+
   Program Definition have_SV ℓ t : dProp Σ :=
-    MonPred (λ TV, ⌜ t ≤ (store_view TV) !!0 ℓ ⌝)%I _.
+    MonPred (λ i, ⌜ t ≤ (store_view i.1) !!0 ℓ ⌝)%I _.
   Next Obligation. solve_proper. Qed.
 
   Global Instance have_SV_persistent ℓ t : Persistent (have_SV ℓ t).
   Proof. apply monPred_persistent=> j. apply _. Qed.
 
   Program Definition have_FV ℓ t : dProp Σ :=
-    MonPred (λ TV, ⌜ t ≤ (flush_view TV) !!0 ℓ ⌝)%I _.
+    MonPred (λ i, ⌜ t ≤ (flush_view i.1) !!0 ℓ ⌝)%I _.
   Next Obligation. solve_proper. Qed.
 
   Global Instance have_FV_persistent ℓ t : Persistent (have_FV ℓ t).
   Proof. apply monPred_persistent=> j. apply _. Qed.
 
   (* This is stronger than [have_FV] when the timestamp is [0]. *)
-  Definition have_FV_strong (ℓ : loc) (t : nat) : dProp Σ :=
-    monPred_in (∅, {[ ℓ := MaxNat t ]}, ∅).
+  Program Definition have_FV_strong (ℓ : loc) (t : nat) : dProp Σ :=
+    have_thread_view (∅, {[ ℓ := MaxNat t ]}, ∅).
+    (* MonPred (λ i, ⌜ {[ ℓ := MaxNat t ]} ⊑ (flush_view i.1) ⌝)%I _. *)
+  (* Next Obligation. solve_proper. Qed. *)
+    (* monPred_in (∅, {[ ℓ := MaxNat t ]}, ∅). *)
 
   Lemma have_SV_0 ℓ : ⊢ have_SV ℓ 0.
   Proof. iModel. iPureIntro. lia. Qed.
@@ -65,7 +89,7 @@ Section definitions.
     have_FV_strong ℓ t -∗ have_FV ℓ t.
   Proof.
     iModel. iPureIntro.
-    destruct TV as [[? FV]?].
+    destruct TV as [[? FV] ?].
     intros [[_ incl] _].
     rewrite /lookup_zero /=.
     apply view_le_singleton in incl as (t2 & -> & le).
@@ -74,19 +98,48 @@ Section definitions.
 
   Lemma monPred_in_have_SV SV PV BV ℓ t :
     t ≤ SV !!0 ℓ →
-    monPred_in (SV, PV, BV) -∗
+    have_thread_view (SV, PV, BV) -∗
     have_SV ℓ t.
   Proof.
     intros le.
-    iStartProof (iProp _). iPureIntro. intros [[SV' ?] ?] [[incl ?]?].
+    iStartProof (iProp _). iPureIntro. intros [[[SV' ?] ?] ?] [[incl ?]?].
     etrans; first done. f_equiv. done.
   Qed.
 
-  Lemma monPred_in_bottom : ⊢@{dPropI Σ} monPred_in (∅, ∅, ∅).
+  Lemma monPred_in_bottom : ⊢@{dPropI Σ} have_thread_view (∅, ∅, ∅).
   Proof.
     iStartProof (iProp _). iPureIntro.
-    intros [[??]?].
+    intros [[[??]?] ?].
     repeat split; apply view_empty_least.
   Qed.
 
+  Program Definition with_gnames (P : nvmDeltaG → dProp Σ) : dProp Σ :=
+    MonPred (λ i, P i.2 i) _.
+  Next Obligation.
+    intros ? [? ?] [? gnames] [? [= ->]].
+    simpl.
+    apply monPred_mono.
+    done.
+  Qed.
+
+  Definition know_gnames (gnames : nvmDeltaG) : dProp Σ :=
+    with_gnames (λ gnames', ⌜ gnames = gnames' ⌝)%I.
+
+  Lemma with_gnames_intro (P : _ → dProp Σ) : (∀ nD, P nD) -∗ with_gnames P.
+  Proof. iModel. iIntros "H". iApply "H". Qed.
+
+  Lemma with_gnames_intro_independent (P : dProp Σ) : P -∗ with_gnames (λ nD, P).
+  Proof. done. Qed.
+
+  Global Instance with_gnames_persistent `{∀ nD, Persistent (P nD)} :
+    Persistent (with_gnames P).
+  Proof.
+    rewrite /Persistent.
+    iModel.
+    simpl.
+    iIntros "#P !>".
+    done.
+  Qed.
+
  End definitions.
+
