src/high/modalities/if_rec.v
@@ -6,29 +6,41 @@ From iris.base_logic Require Import iprop.
 From self.base Require Import primitive_laws wpr_lifting.
 From self.high Require Import dprop resources modalities or_lost monpred_simpl.
 
+Definition crashed_at_d `{nvmBaseFixedG Σ} CV : dProp Σ :=
+  with_gnames (λ nD, ⎡ crashed_at CV ⎤)%I.
+
+Definition persisted_loc_d `{nvmBaseFixedG Σ} ℓ t : dProp Σ :=
+  with_gnames (λ nD, ⎡ persisted_loc ℓ t ⎤)%I.
+
 (* The predicate [P] holds for [ℓ] or [ℓ] has been lost. *)
-Definition if_rec `{nvmBaseFixedG Σ, nvmBaseDeltaG}
+Definition if_rec `{nvmBaseFixedG Σ}
            (ℓ : loc) (P : dProp Σ) : dProp Σ :=
   ∀ (CV : view),
-    ⌜ is_Some (CV !! ℓ) ⌝ -∗ ⎡ crashed_at CV ⎤ -∗ ⎡ persisted_loc ℓ 0 ⎤ -∗ P.
+    ⌜ is_Some (CV !! ℓ) ⌝ -∗ crashed_at_d CV -∗ persisted_loc_d ℓ 0 -∗ P.
 
 (* alt
   P ∨ (∃ CV, ⎡crashed_at CV⎤ ∗ ⌜ℓ ∉ dom (gset _) CV⌝ )
  *)
 
-Class IntoIfRec `{nvmBaseFixedG Σ, nvmBaseDeltaG} ℓ (P : dProp Σ) (Q : dProp Σ) :=
+Class IntoIfRec `{nvmBaseFixedG Σ} ℓ (P : dProp Σ) (Q : dProp Σ) :=
   into_if_rec : P ⊢ if_rec ℓ Q.
-Global Arguments IntoIfRec {_} {_} {_} _ _%I _%I.
-Global Arguments into_if_rec {_} _ _%I _%I.
-Global Hint Mode IntoIfRec ! ! ! + + -  : typeclass_instances.
+Global Arguments IntoIfRec {_} {_} _ _%I _%I.
+Global Arguments into_if_rec {_} _%I _%I.
+Global Hint Mode IntoIfRec ! ! + + -  : typeclass_instances.
 
 Section if_rec.
-  Context `{nvmBaseFixedG Σ, nvmBaseDeltaG}.
+  Context `{nvmBaseFixedG Σ}.
 
-  Local Ltac ifRecIntro := iIntros (CV) "%look #crashed #pers".
+  Local Ltac ifRecIntro :=
+    iIntros (CV);
+    iIntros "%look #crashed #pers".
 
   Lemma if_rec_intro ℓ P : P -∗ if_rec ℓ P.
-  Proof. iIntros "P". ifRecIntro. done. Qed.
+  Proof.
+    iIntros "P".
+    ifRecIntro.
+    done.
+  Qed.
 
   Lemma if_rec_and ℓ P Q : if_rec ℓ (P ∧ Q) ⊣⊢ if_rec ℓ P ∧ if_rec ℓ Q.
   Proof.
@@ -68,7 +80,7 @@ Section if_rec.
   Proof. iIntros "#P". ifRecIntro. iModIntro. iApply "P"; done. Qed.
 
   Lemma modality_if_rec_mixin ℓ :
-    modality_mixin (@if_rec Σ _ _ ℓ)
+    modality_mixin (@if_rec Σ _ ℓ)
       (MIEnvTransform (IntoIfRec ℓ)) (MIEnvTransform (IntoIfRec ℓ)).
   Proof.
     split; simpl; split_and?;
@@ -91,20 +103,20 @@ Section if_rec.
   Global Instance if_rec_proper ℓ : Proper ((⊣⊢) ==> (⊣⊢)) (if_rec (Σ := Σ) ℓ).
   Proof. rewrite /if_rec. intros P Q pToQ. setoid_rewrite pToQ. done. Qed.
 
-  Global Instance if_rec_objective ℓ `{!Objective P} : Objective (if_rec ℓ P).
-  Proof.
-    iIntros (TV1 ?) "P".
-    iIntros (CV ?? look ??) "crashed".
-    iIntros (??) "pers".
-    iSpecialize ("P" $! CV look).
-    monPred_simpl. iSpecialize ("P" $! TV1 with "[//] crashed").
-    monPred_simpl. iSpecialize ("P" $! TV1 with "[//] pers").
-    iApply objective_at.
-    iApply "P".
-  Qed.
+  (* Global Instance if_rec_objective ℓ `{!Objective P} : Objective (if_rec ℓ P). *)
+  (* Proof. *)
+  (*   iIntros (TV1 ?) "P". *)
+  (*   iIntros (CV ?? look ??) "crashed". *)
+  (*   iIntros (??) "pers". *)
+  (*   iSpecialize ("P" $! CV look). *)
+  (*   monPred_simpl. iSpecialize ("P" $! TV1 with "[//] crashed"). *)
+  (*   monPred_simpl. iSpecialize ("P" $! TV1 with "[//] pers"). *)
+  (*   iApply objective_at. *)
+  (*   iApply "P". *)
+  (* Qed. *)
 
   Lemma if_rec_get CV ℓ P :
-    is_Some (CV !! ℓ) → ⎡ crashed_at CV ⎤ -∗ ⎡ persisted_loc ℓ 0 ⎤ -∗ if_rec ℓ P -∗ P.
+    is_Some (CV !! ℓ) → crashed_at_d CV -∗ persisted_loc_d ℓ 0 -∗ if_rec ℓ P -∗ P.
   Proof. iIntros ([[t] look]) "#? #? H". iApply "H"; naive_solver. Qed.
 
   (* Lemma if_rec_with_t_get CV ℓ t P : *)
@@ -119,40 +131,53 @@ Section if_rec.
 
   Lemma if_rec_is_rec ℓ :
     ⊢ if_rec ℓ (∃ CV,
-      ⌜ is_Some (CV !! ℓ) ⌝ ∗ ⎡ crashed_at CV ⎤ ∗ ⎡ persisted_loc ℓ 0 ⎤).
+      ⌜ is_Some (CV !! ℓ) ⌝ ∗ crashed_at_d CV ∗ persisted_loc_d ℓ 0).
   Proof. ifRecIntro. iExists CV. iFrame "#%". Qed.
 
   Lemma if_rec_is_persisted ℓ :
-    ⊢ if_rec ℓ ⎡ persisted_loc ℓ 0 ⎤.
+    ⊢ if_rec ℓ (persisted_loc_d ℓ 0).
   Proof. ifRecIntro. iFrame "#". Qed.
 
-  Lemma or_lost_if_rec_at ℓ (P : dProp Σ) TV :
-    or_lost_post_crash_no_t ℓ (P TV) -∗ (if_rec ℓ P) TV.
+  Lemma or_lost_if_rec_at ℓ (P : dProp Σ) TV nD :
+    or_lost_post_crash_no_t ℓ (P (TV, nD)) -∗ (if_rec ℓ P) (TV, nD).
   Proof.
     iDestruct 1 as (CV) "[crash disj]".
-    iIntros (CV'). monPred_simpl. iIntros (??). monPred_simpl.
-    iIntros ([??] ??). monPred_simpl. iIntros "crashed" (??) "pers".
+    iIntros (CV'). monPred_simpl.
+    iIntros ([??] [? [= <-]]). monPred_simpl.
+    iIntros ([??]). iIntros ([??] [? [= <-]]). monPred_simpl.
+    iIntros "crashed" ([??] [? [= <-]]) "pers".
+    simpl.
     iDestruct (crashed_at_agree with "crash crashed") as %->.
     iApply monPred_mono.
-    2: { iDestruct "disj" as "[(%t & %look & [_ $]) | %]". congruence. }
+    2: { iDestruct "disj" as "[(%t & %look & [_ $]) | %]".
+         congruence. }
+    split; last done.
     etrans; first done. etrans; first done. done.
   Qed.
 
-  Lemma or_lost_if_rec_embed ℓ P TV :
-    or_lost_post_crash_no_t ℓ P -∗ (if_rec ℓ ⎡ P ⎤) TV.
+  Lemma or_lost_if_rec_embed ℓ P TV nD :
+    or_lost_post_crash_no_t ℓ P -∗ (if_rec ℓ ⎡ P ⎤) (TV, nD).
   Proof.
     iIntros "H". iApply or_lost_if_rec_at. rewrite monPred_at_embed. iApply "H".
   Qed.
 
-  Lemma if_rec_or_lost_with_t ℓ P :
-    or_lost_with_t ℓ P -∗ if_rec ℓ (∃ t, P t).
+  Lemma or_lost_if_rec_with_names_embed ℓ P TV nD :
+    or_lost_post_crash_no_t ℓ (P nD) -∗
+    (if_rec ℓ (with_gnames (λ nD', ⎡ P nD' ⎤))) (TV, nD).
   Proof.
-    iIntros "(%CV' & #crashed' & disj)".
-    ifRecIntro. destruct look as [??].
-    iDestruct (crashed_at_agree with "crashed crashed'") as %<-.
-    iDestruct "disj" as "[(% & % & #per & P) | %lost]"; last congruence.
-    iExists t. iFrame "P".
+    iIntros "H". iApply or_lost_if_rec_at.
+    simpl. rewrite monPred_at_embed. iApply "H".
   Qed.
+
+  (* Lemma if_rec_or_lost_with_t ℓ P : *)
+  (*   or_lost_with_t ℓ P -∗ if_rec ℓ (∃ t, P t). *)
+  (* Proof. *)
+  (*   iIntros "(%CV' & #crashed' & disj)". *)
+  (*   ifRecIntro. destruct look as [??]. *)
+  (*   iDestruct (crashed_at_agree with "crashed crashed'") as %<-. *)
+  (*   iDestruct "disj" as "[(% & % & #per & P) | %lost]"; last congruence. *)
+  (*   iExists t. iFrame "P". *)
+  (* Qed. *)
 
   Global Instance into_if_rec_intro ℓ P : IntoIfRec ℓ P P := if_rec_intro ℓ P.
 
