src/high/protocol.v
@@ -4,12 +4,12 @@ From iris_named_props Require Import named_props.
 
 From self Require Import encode_relation.
 From self.high Require Import dprop resources modalities post_crash_modality
-      monpred_simpl or_lost if_rec.
+      monpred_simpl or_lost if_rec predicates.
 From self.lang Require Import lang.
 From self.high.modalities Require Import no_buffer.
 
 (* A handy alias for the type of location predicates. *)
-Definition loc_pred `{nvmG Σ} ST `{AbstractState ST} := ST → val → nvmDeltaG → dProp Σ.
+Definition loc_pred `{nvmG Σ} ST `{AbstractState ST} := ST → val → dProp Σ.
 
 (* A protocol consists of
   - A predicate [pred] that holds for each write and corresponding state of the
@@ -21,9 +21,9 @@ Record LocationProtocol ST `{AbstractState ST, nvmG Σ} := {
   bumper : ST → ST;
   bumper_mono : Proper ((⊑@{ST}) ==> (⊑))%signature bumper;
   pred_condition :
-    (⊢ ∀ (hD : nvmDeltaG) s v,
-      pred s v hD -∗ <PCF> hD', pred (bumper s) v hD' : dProp Σ)%I;
-  pred_nobuf :> (∀ hD s v, IntoNoBuffer (pred s v hD) (pred s v hD));
+    (⊢ ∀ s v,
+      pred s v -∗ <PCF> pred (bumper s) v : dProp Σ)%I;
+  pred_nobuf :> (∀ s v, IntoNoBuffer (pred s v) (pred s v));
 }.
 
 Global Arguments pred {ST} {_} {_} {_} {_} {_} _.
@@ -34,11 +34,11 @@ Existing Instance pred_nobuf.
 
 (** [know_protocol] represents the knowledge that a location is associated with a
 specific protocol. It's defined simply using more "primitive" assertions. *)
-Definition know_protocol `{AbstractState ST, nvmG Σ, nvmDeltaG}
-           ℓ (prot : LocationProtocol ST) : iProp Σ :=
-  "#knowPred" ∷ know_pred ℓ prot.(pred) ∗
-  "#knowPreorder" ∷ know_preorder_loc ℓ (⊑@{ST}) ∗
-  "#knowBumper" ∷ know_bumper ℓ prot.(bumper).
+Definition know_protocol `{AbstractState ST, nvmG Σ}
+           ℓ (prot : LocationProtocol ST) : dProp Σ :=
+  "#knowPred" ∷ know_pred_d ℓ prot.(pred) ∗
+  "#knowPreorder" ∷ know_preorder_loc_d ℓ (⊑@{ST}) ∗
+  "#knowBumper" ∷ know_bumper_d ℓ prot.(bumper).
 
 Lemma encode_bumper_bump_mono `{AbstractState ST}
       (bumper : ST → ST) `{!Proper ((⊑@{ST}) ==> (⊑))%signature bumper}
@@ -61,22 +61,26 @@ Section protocol.
   Implicit Types (prot : LocationProtocol ST).
 
   Lemma post_crash_know_protocol ℓ prot :
-    ⎡ know_protocol ℓ prot ⎤ -∗ <PC> hD, if_rec ℓ (⎡ know_protocol ℓ prot ⎤).
-  Proof. iIntros "(a & b & c)". iCrash. iModIntro. iFrame. Qed.
+    know_protocol ℓ prot -∗ <PC> if_rec ℓ (know_protocol ℓ prot).
+  Proof.
+    iIntros "(a & b & c)".
+    iDestruct (post_crash_know_pred with "a") as "a".
+    iCrash. iModIntro. iFrame.
+  Qed.
 
   Global Instance know_protocol_into_crash ℓ prot :
     IntoCrash
-      (⎡ know_protocol ℓ prot ⎤)%I
-      (λ hG', if_rec ℓ (⎡ know_protocol ℓ prot ⎤))%I.
+      (know_protocol ℓ prot)
+      (if_rec ℓ (know_protocol ℓ prot)).
   Proof.
     rewrite /IntoCrash. iIntros "P". by iApply post_crash_know_protocol.
   Qed.
 
   Lemma know_protocol_extract ℓ prot :
     know_protocol ℓ prot -∗
-      know_pred ℓ prot.(pred) ∗
-      know_preorder_loc ℓ (⊑@{ST}) ∗
-      know_bumper ℓ prot.(bumper).
+      know_pred_d ℓ prot.(pred) ∗
+      know_preorder_loc_d ℓ (⊑@{ST}) ∗
+      know_bumper_d ℓ prot.(bumper).
   Proof. iNamed 1. iFrame "#". Qed.
 
 End protocol.
